CCsub_Soundness.v
@@ -13,11 +13,13 @@ Hint Constructors store_typing eval_typing state_typing : core.
 (* ********************************************************************** *)
 (** * #<a name="preservation"></a># Preservation *)
 
-Definition no_type_bindings (Γ : env) : Prop :=
-  forall X U, ~ binds X (bind_sub U) Γ.
+(* Definition no_type_bindings (Γ : store_env) : Prop := *)
+(*   forall X U, ~ Store.binds X (bind_sub U) Γ. *)
 
+(* Should be true because of new definitions *)
+(*
 Lemma store_typing_no_type_bindings : forall S Γ,
-  S ∷ Γ ->
+  store_typing S Γ ->
   no_type_bindings Γ.
 Proof with eauto*.
   intros * StoreTyp.
@@ -28,109 +30,109 @@ Proof with eauto*.
     rename select (binds _ (bind_sub _) _) into Binds.
     applys IHStoreTyp Binds.
 Qed.
+*)
 
-Lemma stores_implies_value : forall S Γ x v,
-  S ∷ Γ ->
-  stores S x v ->
+Lemma env_implies_value : forall S E l v,
+  store_typing E S ->
+  stores E l v ->
   value v.
 Proof with eauto*.
   intros * StoreTyp Stores.
   induction StoreTyp; inversion Stores; subst.
-  destruct (x == x0); subst...
+  destruct (l ==== l0); subst...
 Qed.
 
-Lemma stores_preserves_typing : forall S Γ x v C P,
-  S ∷ Γ ->
-  stores S x v ->
-  Γ ⊢ x : (C # P) ->
-  exists D Q, Γ ⊢ v : (exp_cv v # Q)
-         /\ binds x (bind_typ (D # Q)) Γ
-         /\ Γ ⊢ₛ (exp_cv v) <: D
-         /\ Γ ⊢ Q <: P.
+Lemma stores_preserves_typing : forall S E l v C P,
+  store_typing E S ->
+  stores E l v ->
+  typing nil S l (C # P) ->
+  exists D Q, typing nil S v (exp_cv v # Q)
+         /\ Store.binds l (D # Q) S
+         /\ subcapt nil S (exp_cv v) D
+         /\ sub nil S Q P.
 Proof with eauto*.
-  intros * StoreTyp xStores.
+  intros * StoreTyp lStores.
   revert C P.
-  induction StoreTyp as [|y D Q w S Γ StoreTyp IH w_value Typ NotIn]; intros C P Typ'; inversion xStores.
-  assert (WfEnv' : ([(y, bind_typ (D # Q))] ++ Γ) ⊢ wf) by applys typing_regular Typ'.
-  assert (WfEnv : Γ ⊢ wf) by (inversion WfEnv'; auto).
-  assert (WfQ : Γ ⊢ Q wf) by (inversion WfEnv'; eauto* ).
-  assert (WfQ' : ([(y, bind_typ (D # Q))] ++ Γ) ⊢ Q wf) by (rewrite_nil_concat; apply wf_typ_weakening; eauto* ).
-  destruct (x == y); subst.
-  - Case "x = y".
+  induction StoreTyp as [|y D Q w E S StoreTyp IH w_value Typ NotIn]; intros C P Typ'; inversion lStores.
+  destruct (l ==== y); subst.
+  - Case "l = y".
     inversion select (Some _ = Some _); subst.
-    destruct (values_have_precise_captures _ _ _ _ w_value Typ) as [U [TypCVU CVUSubDQ]].
-    exists D, Q. 
+    destruct (values_have_precise_captures _ _ _ _ S w_value Typ) as [U [TypCVU CVUSubDQ]].
+    exists D, Q.
     inversion CVUSubDQ; subst.
     repeat split...
-    + rewrite_nil_concat.
-      apply typing_weakening...
-      apply typing_sub with (S := exp_cv v # U)...
-      apply sub_capt...
-      apply subcapt_reflexivity...
-    + rewrite_nil_concat.
-      apply subcapt_weakening...
+    + inversion CVUSubDQ; subst...
+      assert (typing nil S v (exp_cv v # Q)). {
+        apply typing_sub with (R := exp_cv v # U).
+        assumption.
+        inversion CVUSubDQ; subst...
+        apply sub_capt...
+        apply subcapt_reflexivity...
+      }
+      rewrite_env (nil ++ [(y, D # Q)] ++ S).
+      apply typing_weakening_store...
+    + rewrite Store.cons_concat.
+      apply Store.binds_head.
+      apply Store.binds_singleton.
+    + rewrite_env (nil ++ [(y, D # Q)] ++ S).
+      apply subcapt_weakening_store...
     + eremember (C # P) as T.
-      assert (Sub : ([(y, bind_typ (D # Q))] ++ Γ) ⊢ T <: (C # P)).
-      { rewrite HeqT in Typ' |- *; apply sub_reflexivity.
-        - apply WfEnv'.
-        - applys typing_regular Typ'.
+      assert (Sub : sub nil ([(y, D # Q)] ++ S) T (C # P)). {
+        rewrite <- HeqT.
+        apply sub_reflexivity...
       }
       clear HeqT.
       dependent induction Typ'.
-      * rename select (binds _ _ _) into Binds.
-        binds_cases Binds.
-        -- simpl in Fr; exfalso; fsetdec.
-        -- inversion select (bind_typ _ = bind_typ _); subst.
-           inversion select (_ ⊢ (_ # Q) <: (_ # P)); subst...
+      * rename select (Store.binds _ _ _) into Binds.
+        assert (C0 # R = D # Q). {
+          apply Store.binds_mid_eq_cons with (x := y) (F := nil) (E := S)...
+        }
+        Store.binds_cases Binds.
+        inversion H0; subst...
+        inversion Sub...
       * eapply IHTyp'...
         apply sub_transitivity with (Q := T)...
-  - Case "x <> y".
-    destruct (typing_var_implies_binds_typ _ _ _ _ Typ') as [C' [R' [Binds [WfC [WfC' [WfR' PureR']]]]]].
-    assert (Binds' : binds x (bind_typ (C' # R')) Γ) by (binds_cases Binds; eauto* ).
-    assert (WfC'R' : Γ ⊢ (C' # R') wf).
-    { destruct (wf_typ_env_bind_typ x (C' # R') Γ ltac:(inversion WfEnv'; auto) Binds') as [C'' [R'' [Eq'' WfC''R'']]].
-      symmetry in Eq''; inversion Eq''; subst; clear Eq''...
-    }
+  - Case "l <> y".
+    destruct (typing_loc_implies_binds _ _ _ _ _ Typ') as [C' [R' [Binds Rest]]].
+    assert (Binds' : Store.binds l (C' # R') S) by (eapply Store.binds_remove_mid_cons with (G := nil); eauto).
+    assert (WfC'R' : wf_typ nil S (C' # R')) by (apply wf_typ_from_wf_store_ctx with (l := l); eauto).
     destruct (IH ltac:(assumption) C' R') as [D'' [Q'' [Typ'' [Binds'' [CVsubD'' Q''subR']]]]].
-    + apply typing_sub with (S := `cset_fvar` x # R').
-      * eapply typing_var...
-      * apply sub_capt...
-        -- eapply subcapt_var...
-           apply subcapt_reflexivity.
-           inversion WfC'R'...
+    + apply typing_sub with (R := cse_loc l # R').
+      * apply typing_loc with (C := C')...
+      * apply sub_capt; try inversion WfC'R'; subst...
+        -- apply (subcapt_trans_loc _ C' _ _ _ R')...
+           apply subcapt_reflexivity...
         -- apply sub_reflexivity...
-        -- applys sub_pure_type...
-        -- applys sub_pure_type...
-    + assert (Eq : bind_typ (C' # R') = bind_typ (D'' # Q'')).
-      { eapply binds_unique... }
+    + assert (Eq : (C' # R') = (D'' # Q'')).
+      { apply Store.binds_unique with (E := S) (x := l)... }
       symmetry in Eq; inversion Eq; subst.
       exists C', R'.
       repeat split...
-      * rewrite_nil_concat.
-        apply typing_weakening...
-      * rewrite_nil_concat.
-        apply subcapt_weakening...
+      * rewrite_env (nil ++ [(y, D # Q)] ++ S).
+        apply typing_weakening_store...
+      * rewrite_env (nil ++ [(y, D # Q)] ++ S).
+        apply subcapt_weakening_store...
 Qed.
 
-Lemma eval_typing_sub : forall Γ K S1 S2 T1 T2,
-  Γ ⊢ S2 <: S1 ->
-  Γ ⊢ K : S1 ⇒ T1 ->
-  Γ ⊢ T1 <: T2 ->
-  Γ ⊢ K : S2 ⇒ T2.
+Lemma eval_typing_sub : forall Γ S K R1 R2 T1 T2,
+  sub Γ S R2 R1 ->
+  eval_typing Γ S K R1 T1 ->
+  sub Γ S T1 T2 ->
+  eval_typing Γ S K R2 T2.
 Proof with eauto*.
-  intros * S2SubS1 EvalTyp T1SubT2.
-  revert S2 T2 S2SubS1 T1SubT2.
-  induction EvalTyp; intros S2 T2 S2subC1R1 C2R2subT2.
+  intros * R2SubR1 EvalTyp T1SubT2.
+  revert R2 T2 R2SubR1 T1SubT2.
+  induction EvalTyp; intros R4 T2 R2subC1R1 C2R2subT2.
   - Case "typing_eval_nil".
-    rename select (Γ ⊢ (C1 # R1) <: (C2 # R2)) into C1R1subC2R2.
-    destruct (proj1 (sub_capt_type _ _ _ C2R2subT2) ltac:(eauto)) as [D2 [Q2 Eq]]; subst.
-    destruct (proj2 (sub_capt_type _ _ _ S2subC1R1) ltac:(eauto)) as [D1 [Q1 Eq]]; subst.
+    rename select (sub Γ S (C1 # R1) (C2 # R2)) into C1R1subC2R2.
+    destruct (proj1 (sub_capt_type _ _ _ _ C2R2subT2) ltac:(eauto)) as [D2 [Q2 Eq]]; subst.
+    destruct (proj2 (sub_capt_type _ _ _ _ R2subC1R1) ltac:(eauto)) as [D1 [Q1 Eq]]; subst.
     apply typing_eval_nil...
     apply sub_transitivity with (Q := C1 # R1)...
     apply sub_transitivity with (Q := C2 # R2)...
   - Case "typing_eval_cons".  
-    destruct (proj1 (sub_capt_type _ _ _ C2R2subT2) ltac:(eauto)) as [D2 [Q2 Eq]]; subst.
-    destruct (proj2 (sub_capt_type _ _ _ S2subC1R1) ltac:(eauto)) as [D1 [Q1 Eq]]; subst.
+    destruct (proj1 (sub_capt_type _ _ _ _ C2R2subT2) ltac:(eauto)) as [D2 [Q2 Eq]]; subst.
+    destruct (proj2 (sub_capt_type _ _ _ _ R2subC1R1) ltac:(eauto)) as [D1 [Q1 Eq]]; subst.
     apply typing_eval_cons with (L := L) (C2 := C2) (R2 := R2)...
     + intros x xNotIn.
       rewrite_nil_concat.
@@ -140,12 +142,12 @@ Proof with eauto*.
       applys eval_typing_regular EvalTyp.
 Qed.
 
-Lemma eval_typing_weakening : forall Γ Δ Θ E T U,
-  (Δ ++ Γ) ⊢ E : T ⇒ U ->
-  (Δ ++ Θ ++ Γ) ⊢ wf ->
-  (Δ ++ Θ ++ Γ) ⊢ E : T ⇒ U.
+Lemma eval_typing_weakening : forall Γ Δ Θ S E T U,
+  eval_typing (Δ ++ Γ) S E T U ->
+  wf_ctx (Δ ++ Θ ++ Γ) S ->
+  eval_typing (Δ ++ Θ ++ Γ) S E T U.
 Proof with eauto*.
-  intros * EvalTyp WfEnv.
+  intros * EvalTyp WfCtx.
   induction EvalTyp.
   - Case "typing_eval_nil".
     apply typing_eval_nil...
@@ -153,21 +155,38 @@ Proof with eauto*.
   - Case "typing_eval_cons".
     apply typing_eval_cons with (L := L `u`A dom (Δ ++ Θ ++ Γ)) (C2 := C2) (R2 := R2)...
     intros x xNotIn.
-    rename select (forall x, x ∉ L -> _ ⊢ _ : _) into Typ.
+    rename select (forall x, x ∉ L -> typing _ _ _ _) into Typ.
     specialize (Typ x ltac:(fsetdec)).
     rewrite <- concat_assoc in Typ.
     apply typing_weakening with (Θ := Θ) in Typ.
     + apply Typ.
     + simpl_env.
-      apply wf_env_typ...
-      assert (WfEnv' : (([(x, bind_typ (C1 # R1))] ++ Δ) ++ Γ) ⊢ wf) by applys typing_regular Typ.
-      inversion WfEnv'; subst.
+      apply wf_ctx_typ...
+      assert (WfCtx' : wf_ctx (([(x, bind_typ (C1 # R1))] ++ Δ) ++ Γ) S) by applys typing_regular Typ.
+      inversion WfCtx'; subst.
       apply wf_typ_weakening...
 Qed.
 
-Lemma store_typing_preserves_dom : forall S Γ,
-  S ∷ Γ ->
-  dom S = dom Γ.
+Lemma eval_typing_weakening_store : forall Γ S1 S2 S3 E T U,
+  eval_typing Γ (S1 ++ S2) E T U ->
+  wf_store_ctx (S1 ++ S3 ++ S2) ->
+  eval_typing Γ (S1 ++ S3 ++ S2) E T U.
+Proof with eauto*.
+  intros * EvalTyp WfCtx.
+  induction EvalTyp.
+  - Case "typing_eval_nil".
+    apply typing_eval_nil...
+    apply sub_weakening_store...
+  - Case "typing_eval_cons".
+    apply typing_eval_cons with (L := L) (C2 := C2) (R2 := R2)...
+    intros x xNotIn.
+    specialize (H x xNotIn).
+    apply typing_weakening_store with (S2 := S3) in H...
+Qed.
+
+Lemma store_typing_preserves_dom : forall E S,
+  store_typing E S ->
+  Store.dom E = Store.dom S.
 Proof with eauto*.
   intros * StoreTyp.
   induction StoreTyp...
@@ -175,144 +194,156 @@ Proof with eauto*.
   rewrite IHStoreTyp...
 Qed.
 
-Lemma typing_inv_app : forall Γ (f x : atom) T,
-  Γ ⊢ (f @ x) : T ->
-  exists C D Q U, Γ ⊢ f : (C # (∀ (D # Q) U))
-               /\ Γ ⊢ x : (D # Q)
-               /\ Γ ⊢ (open_ct U (`cset_fvar` x)) <: T.
+Lemma typing_inv_app : forall Γ S (f x : atom) T,
+  typing Γ S (f @ x) T ->
+  exists C D Q U, typing Γ S f (C # (∀ (D # Q) U))
+               /\ typing Γ S x (D # Q)
+               /\ sub Γ S (open_ct U (cse_fvar x)) T.
 Proof with eauto*.
   intros * Typ.
-  forwards (WfEnv & _ & WfT): typing_regular Typ.
+  forwards (WfStore & WfCtx & _ & WfT): typing_regular Typ.
   dependent induction Typ.
   - Case "typing_app".
     repeat eexists...
     apply sub_reflexivity...
   - Case "typing_sub".
-    rename select (Γ ⊢ S <: T) into Sub.
-    assert (WfS : Γ ⊢ S wf) by applys sub_regular Sub.
-    destruct (IHTyp f x ltac:(reflexivity) WfEnv WfS) as [C [D [Q [U [fTyp [xTyp Sub']]]]]].
+    rename select (sub Γ S R T) into Sub.
+    assert (WfR : wf_typ Γ S R) by applys sub_regular Sub.
+    destruct (IHTyp f x ltac:(reflexivity) WfStore WfCtx WfR) as [C [D [Q [U [fTyp [xTyp Sub']]]]]].
     repeat eexists...
-    apply sub_transitivity with (Q := S)...
+    apply sub_transitivity with (Q := R)...
 Qed.
 
-Lemma typing_inv_tapp : forall Γ (x : atom) V T,
-  Γ ⊢ (x @ [V]) : T ->
-  exists C R U, Γ ⊢ x : (C # (∀ [R] U))
-             /\ Γ ⊢ V <: R
-             /\ Γ ⊢ (open_tt U V) <: T.
-Proof with eauto*.
-  intros * Typ.
-  dependent induction Typ.
-  - Case "typing_tapp".
-    exists C, Q, T.
-    repeat split...
-    forwards (WfEnv & _ & WfCQT): typing_regular Typ.
-    inversion WfCQT; subst.
-    apply sub_reflexivity.
-    1: assumption.
-    inversion select (Γ ⊢ (∀ [Q] T) wf); subst.
-    rename select (forall X : atom, X ∉ L -> _ ⊢ _ wf) into WfT.
-    pick fresh Y and specialize WfT.
-    replace (open_tt T V)
-       with (subst_tt Y V (open_tt T Y))
-         by (symmetry; apply subst_tt_intro; fsetdec).
-         rewrite_env (map (subst_tb Y V) ∅ ++ Γ).
-    eapply wf_typ_subst_tb...
-    + applys sub_pure_type...
-    + apply ok_cons...
-  - Case "typing_sub".
-    destruct (IHTyp x V eq_refl) as [C [R [U [fTyp [xTyp Sub]]]]].
-    exists C, R, U.
-    repeat split...
-    apply sub_transitivity with (Q := S)...
-Qed.
+(* Lemma typing_inv_tapp : forall Γ (x : atom) V T, *)
+(*   Γ ⊢ (x @ [V]) : T -> *)
+(*   exists C R U, Γ ⊢ x : (C # (∀ [R] U)) *)
+(*              /\ Γ ⊢ V <: R *)
+(*              /\ Γ ⊢ (open_tt U V) <: T. *)
+(* Proof with eauto*. *)
+(*   intros * Typ. *)
+(*   dependent induction Typ. *)
+(*   - Case "typing_tapp". *)
+(*     exists C, Q, T. *)
+(*     repeat split... *)
+(*     forwards (WfEnv & _ & WfCQT): typing_regular Typ. *)
+(*     inversion WfCQT; subst. *)
+(*     apply sub_reflexivity. *)
+(*     1: assumption. *)
+(*     inversion select (Γ ⊢ (∀ [Q] T) wf); subst. *)
+(*     rename select (forall X : atom, X ∉ L -> _ ⊢ _ wf) into WfT. *)
+(*     pick fresh Y and specialize WfT. *)
+(*     replace (open_tt T V) *)
+(*        with (subst_tt Y V (open_tt T Y)) *)
+(*          by (symmetry; apply subst_tt_intro; fsetdec). *)
+(*          rewrite_env (map (subst_tb Y V) ∅ ++ Γ). *)
+(*     eapply wf_typ_subst_tb... *)
+(*     + applys sub_pure_type... *)
+(*     + apply ok_cons... *)
+(*   - Case "typing_sub". *)
+(*     destruct (IHTyp x V eq_refl) as [C [R [U [fTyp [xTyp Sub]]]]]. *)
+(*     exists C, R, U. *)
+(*     repeat split... *)
+(*     apply sub_transitivity with (Q := S)... *)
+(* Qed. *)
+(**)
+(* Lemma typing_inv_box : forall Γ x T, *)
+(*   Γ ⊢ (box x) : T -> *)
+(*   exists C R, Γ ⊢ x : (C # R) *)
+(*            /\ `cset_fvars` C ⊆ dom Γ *)
+(*            /\ Γ ⊢ ({} # □ (C # R)) <: T. *)
+(* Proof with eauto*. *)
+(*   intros * Typ. *)
+(*   forwards (WfEnv & _ & WfT): typing_regular Typ. *)
+(*   dependent induction Typ... *)
+(*   - Case "typing_box". *)
+(*     exists C, R. *)
+(*     repeat split... *)
+(*     apply sub_reflexivity... *)
+(*   - Case "typing_sub". *)
+(*     rename select (Γ ⊢ S <: T) into Sub. *)
+(*     assert (WfS : Γ ⊢ S wf) by applys sub_regular Sub. *)
+(*     destruct (IHTyp x eq_refl WfEnv WfS) as [C [R [xTyp [xSubΓ CRsubS]]]]. *)
+(*     exists C, R. *)
+(*     repeat split... *)
+(*     apply sub_transitivity with (Q := S)... *)
+(* Qed. *)
+(**)
+(* Lemma typing_inv_unbox : forall Γ C x T, *)
+(*   Γ ⊢ (C ⟜ x) : T -> *)
+(*   exists R, Γ ⊢ x : ({} # (□ (C # R))) *)
+(*          /\ Γ ⊢ (C # R) <: T. *)
+(* Proof with eauto*. *)
+(*   intros * Typ. *)
+(*   forwards (WfEnv & _ & WfT): typing_regular Typ. *)
+(*   dependent induction Typ... *)
+(*   - Case "typing_unbox". *)
+(*     exists R. *)
+(*     repeat split... *)
+(*     apply sub_reflexivity... *)
+(*   - Case "typing_sub". *)
+(*     rename select (Γ ⊢ S <: T) into Sub. *)
+(*     assert (WfS : Γ ⊢ S wf) by applys sub_regular Sub. *)
+(*     destruct (IHTyp _ _ eq_refl WfEnv WfS) as [R [xTyp CRsubS]]. *)
+(*     exists R. *)
+(*     repeat split... *)
+(*     apply sub_transitivity with (Q := S)... *)
+(* Qed. *)
 
-Lemma typing_inv_box : forall Γ x T,
-  Γ ⊢ (box x) : T ->
-  exists C R, Γ ⊢ x : (C # R)
-           /\ `cset_fvars` C ⊆ dom Γ
-           /\ Γ ⊢ ({} # □ (C # R)) <: T.
-Proof with eauto*.
-  intros * Typ.
-  forwards (WfEnv & _ & WfT): typing_regular Typ.
-  dependent induction Typ...
-  - Case "typing_box".
-    exists C, R.
-    repeat split...
-    apply sub_reflexivity...
-  - Case "typing_sub".
-    rename select (Γ ⊢ S <: T) into Sub.
-    assert (WfS : Γ ⊢ S wf) by applys sub_regular Sub.
-    destruct (IHTyp x eq_refl WfEnv WfS) as [C [R [xTyp [xSubΓ CRsubS]]]].
-    exists C, R.
-    repeat split...
-    apply sub_transitivity with (Q := S)...
-Qed.
-
-Lemma typing_inv_unbox : forall Γ C x T,
-  Γ ⊢ (C ⟜ x) : T ->
-  exists R, Γ ⊢ x : ({} # (□ (C # R)))
-         /\ Γ ⊢ (C # R) <: T.
-Proof with eauto*.
-  intros * Typ.
-  forwards (WfEnv & _ & WfT): typing_regular Typ.
-  dependent induction Typ...
-  - Case "typing_unbox".
-    exists R.
-    repeat split...
-    apply sub_reflexivity...
-  - Case "typing_sub".
-    rename select (Γ ⊢ S <: T) into Sub.
-    assert (WfS : Γ ⊢ S wf) by applys sub_regular Sub.
-    destruct (IHTyp _ _ eq_refl WfEnv WfS) as [R [xTyp CRsubS]].
-    exists R.
-    repeat split...
-    apply sub_transitivity with (Q := S)...
-Qed.
+(* Lemma binds_implies_typing : forall Γ S l C R, *)
+(*   wf_ctx Γ S -> *)
+(*   wf_typ Γ S (C # R) -> *)
+(*   l `Notin` Store.dom S -> *)
+(*   wf_store_ctx ([(l, (C # R))] ++ S) -> *)
+(*   typing Γ ([(l, (C # R))] ++ S) l (C # R). *)
+(* Proof with eauto*. *)
+(*   intros * WfCtx WfCR NotIn WfStore. *)
+(*   dependent induction WfStore... *)
+(*   Unset Printing Notations. *)
+(*   assert (S ~= [(l, (C # R))] ++ S). { *)
+(*   enough (S <> [(l, (C # R))] ++ S). { *)
+(**)
+(*   } *)
+(*    *)
+(*   } *)
+(*   specialize (IHWfStore R C l S WfCtx WfCR NotIn ltac:(eauto))... *)
 
 Lemma preservation : forall Σ Σ' V,
   state_typing Σ V ->
   Σ --> Σ' ->
   state_typing Σ' V.
 Proof with eauto*.
-  intros * [S Γ E e C1 R1 C2 R2 StoreTyp EvalTyp Typ] Red.
-  forwards (WfEnv & WfC1R1 & WfC2R2): eval_typing_regular EvalTyp.
+  intros * [S E e C1 R1 C2 R2 v Typ EvalTyp] Red.
+  forwards (WfStore & WfCtx & WfC1R1 & WfC2R2): eval_typing_regular EvalTyp.
   dependent induction Red.
   - Case "red_lift".
     inversion EvalTyp; subst.
-    rename select (forall x, x ∉ L -> _ ⊢ _ : _) into Typ'.
-    eapply typing_state with (Γ := [(x, bind_typ (C1 # R1))] ++ Γ).
+    rename select (forall x, x ∉ L -> typing _ _ _ _) into Typ'.
+    eapply typing_state with (S := [(l, (C1 # R1))] ++ S).
     + apply typing_store_cons...
-      rewrite <- store_typing_preserves_dom with (S := S)...
-    + rewrite_nil_concat.
-      apply eval_typing_weakening...
-      apply wf_env_typ...
-      rewrite <- store_typing_preserves_dom with (S := S)...
+      rewrite <- store_typing_preserves_dom with (E := E)...
+    + Store.rewrite_nil_concat.
+      apply eval_typing_weakening_store...
+      simpl. constructor...
+      rewrite <- store_typing_preserves_dom with (E := E)...
     + pick fresh y and specialize Typ'.
-      assert (x ∉ dom Γ) by (rewrite <- store_typing_preserves_dom with (S := S); assumption).
-      assert (WfEnv' : ([(x, bind_typ (C1 # R1))] ++ Γ) ⊢ wf) by (apply wf_env_typ; eauto* ).
-      eapply typing_through_open_ve_typing with (y := y) (U := C1 # R1).
+      assert (l `Notin` Store.dom S) by (rewrite <- store_typing_preserves_dom with (E := E); assumption).
+      assert (WfStore' : wf_store_ctx ([(l, (C1 # R1))] ++ S)) by (constructor; eauto*).
+      eapply typing_through_open_ve_typing_loc with (y := y) (U := C1 # R1).
       * simpl; clear - Fr; fsetdec.
-      * apply typing_weakening.
+      * Store.rewrite_nil_concat. apply typing_weakening_store.
         1: assumption.
-        repeat apply wf_env_typ...
-        apply wf_typ_weaken_head...
-      * apply typing_sub with (S := `cset_fvar` x # R1).
-        1: apply typing_var with (C := C1)...
-        apply sub_capt.
-        -- eapply subcapt_var...
-           apply subcapt_reflexivity.
-           apply wf_cset_weaken_head...
-        -- apply sub_reflexivity...
-           apply wf_typ_weaken_head...
-        -- inversion WfC1R1; subst...
-        -- inversion WfC1R1; subst...
+        eauto.
+      * apply typing_sub with (R := (cse_loc l # R1))...
+        assert (pure_type R1) by (inversion WfC1R1; eauto).
+        constructor...
+        constructor.
+
   - Case "red_let_var".
     inversion EvalTyp; subst.
-    rename select (forall x, x ∉ L -> _ ⊢ _ : _) into Typ'.
-    eapply typing_state with (Γ := Γ)...
+    rename select (forall x, x ∉ L -> typing _ _ _ _) into Typ'.
+    eapply typing_state with (StoreEnv := E)...
     pick fresh y and specialize Typ'.
-    eapply typing_through_open_ve_typing with (y := y)...
+    eapply typing_through_open_ve_typing_loc with (y := y)...
   - Case "red_let_val".
     destruct (typing_inv_let _ _ _ _ Typ) as [D [Q [vTyp [L kTyp]]]].
     assert (x ∉ dom Γ) by (rewrite <- store_typing_preserves_dom with (S := S); assumption).
